Implement monadic pairs and lists, #37

Coq/src/Effect.v
@@ -8,7 +8,11 @@ Definition NDShare := C__Comb (C__State nat) (C__Comb C__Sharing C__Choice).
 
 Definition NDShare__SC := C__Comb C__Sharing C__Choice.
 
-Definition Fail A : Free NDShare A :=
+Definition Prog := Free NDShare.
+
+Definition Prog__SC := Free NDShare__SC.
+
+Definition Fail A : Prog A :=
   let s : @Shape _ NDShare := inr (inr sfail)
   in impure (ext s (fun p : @Pos _ NDShare s => match p with end)).
 
@@ -26,33 +30,33 @@ Definition Fail__SC A : Free (C__Comb C__Sharing C__Choice) A :=
 
 Arguments Fail__SC {_}.
 
-Definition Get : Free NDShare nat :=
+Definition Get : Prog nat :=
   let s : @Shape _ NDShare := inl (sget nat)
   in impure (ext s (fun p : @Pos _ NDShare s => match p with pget s => pure s end)).
 
-Definition Put (n : nat) : Free NDShare unit :=
+Definition Put (n : nat) : Prog unit :=
   let s : @Shape _ NDShare := inl (sput n)
   in impure (ext s (fun p : @Pos _ NDShare s => match p with pput s => pure tt end)).
 
-Definition Share' (n : nat) A (fs : Free NDShare A) : Free NDShare A :=
+Definition Share' (n : nat) A (fs : Prog A) : Prog A :=
   let s : @Shape _ NDShare := inr (inl (ssharing n))
   in impure (ext s (fun p : @Pos _ NDShare s => fs)).
 
-Definition Share'__SC (n : nat) A (fs : Free NDShare__SC A) : Free NDShare__SC A :=
+Definition Share'__SC (n : nat) A (fs : Prog__SC A) : Prog__SC A :=
   let s : @Shape _ NDShare__SC := inl (ssharing n)
   in impure (ext s (fun p : @Pos _ NDShare__SC s => fs)).
 
-Definition Share A (fp : Free NDShare A) : Free NDShare (Free NDShare A) :=
+Definition Share A (fp : Prog A) : Prog (Prog A) :=
   Get >>= fun i => Put (i * 2) >>= fun _=> pure (Share' i (Put (i * 2 + 1) >>= fun _ => fp)).
 
 Definition Choice__C A mid l r : Free C__Choice A :=
   let s : @Shape _ C__Choice := schoice mid
   in impure (ext s (fun p : Pos__Choice s => if p then l else r)).
 
-Definition Choice__SC A mid l r : Free NDShare__SC A :=
+Definition Choice__SC A mid l r : Prog__SC A :=
   let s : @Shape _ NDShare__SC := inr (schoice mid)
   in impure (ext s (fun p : @Pos _ NDShare__SC s => if p then l else r)).
 
-Definition Choice A mid l r : Free NDShare A :=
+Definition Choice A mid l r : Prog A :=
   let s : @Shape _ NDShare := inr (inr (schoice mid))
   in impure (ext s (fun p : @Pos _ NDShare s => if p then l else r)).
